theories/tmc_2/definition.v
@@ -1,0 +1,275 @@
+From camlcert Require Import
+  prelude.
+From camlcert.data_lang Require Export
+  syntax.
+From camlcert.data_lang Require Import
+  notations.
+From camlcert Require Import
+  options.
+
+Implicit Types func func_dps : data_function.
+Implicit Types annot : data_annotation.
+Implicit Types v vₛ vₜ : data_val.
+Implicit Types e eₛ eₜ : data_expr.
+Implicit Types prog progₛ progₜ : data_program.
+
+Definition tmc_mapping :=
+  gmap data_function data_function.
+
+Inductive tmc_side :=
+  | TmcLeft
+  | TmcRight.
+
+Coercion tmc_side_to_index side :=
+  match side with
+  | TmcLeft =>
+      𝟙
+  | TmcRight =>
+      𝟚
+  end.
+Definition tmc_side_invert side :=
+  match side with
+  | TmcLeft =>
+      TmcRight
+  | TmcRight =>
+      TmcLeft
+  end.
+
+Record tmc_ctxi := TmcCtxi {
+  tmc_ctxi_tag : data_tag ;
+  tmc_ctxi_side : tmc_side ;
+  tmc_ctxi_expr : data_expr ;
+}.
+Add Printing Constructor tmc_ctxi.
+Implicit Types c : tmc_ctxi.
+
+#[global] Instance tmc_ctxi_fill : Fill tmc_ctxi data_expr :=
+  Build_Fill (λ c e,
+    match c.(tmc_ctxi_side) with
+    | TmcLeft =>
+        &c.(tmc_ctxi_tag) e c.(tmc_ctxi_expr)
+    | TmcRight =>
+        &c.(tmc_ctxi_tag) c.(tmc_ctxi_expr) e
+    end
+  )%data_expr.
+#[global] Instance tmc_ctxi_hsubst : HSubst data_expr tmc_ctxi :=
+  λ ς c,
+    TmcCtxi c.(tmc_ctxi_tag) c.(tmc_ctxi_side) c.(tmc_ctxi_expr).[ς].
+
+Definition tmc_ctx :=
+  list tmc_ctxi.
+Implicit Types C : tmc_ctx.
+
+#[global] Instance tmc_ctx_fill : Fill tmc_ctx data_expr :=
+  Build_Fill (λ C e,
+    foldl (λ e c, c @@ e) e C
+  ).
+#[global] Instance tmc_ctx_hsubst : HSubst data_expr tmc_ctx :=
+  λ ς C,
+    (hsubst ς) <$> C.
+
+Record tmc_rctxi := TmcRctxi {
+  tmc_rctxi_tag : data_tag ;
+  tmc_rctxi_side : tmc_side ;
+  tmc_rctxi_val : data_val ;
+}.
+Add Printing Constructor tmc_rctxi.
+
+Coercion tmc_rctxi_to_ctxi (c : tmc_rctxi) :=
+  TmcCtxi c.(tmc_rctxi_tag) c.(tmc_rctxi_side) c.(tmc_rctxi_val).
+
+Definition tmc_rctx :=
+  list tmc_rctxi.
+
+Definition tmc_rctx_to_ctx : tmc_rctx → tmc_ctx :=
+  fmap tmc_rctxi_to_ctxi.
+Coercion tmc_rctx_to_ctx : tmc_rctx >-> tmc_ctx.
+
+Section tmc_expr.
+  Context (ξ : tmc_mapping).
+
+  Inductive tmc_expr_dir : data_expr → data_expr → Prop :=
+    | tmc_expr_dir_val v :
+        tmc_expr_dir
+          v
+          v
+    | tmc_expr_dir_var x :
+        tmc_expr_dir
+          $x
+          $x
+    | tmc_expr_dir_let eₛ1 eₛ2 eₜ1 eₜ2 :
+        tmc_expr_dir eₛ1 eₜ1 →
+        tmc_expr_dir eₛ2 eₜ2 →
+        tmc_expr_dir
+          (let: eₛ1 in eₛ2)
+          (let: eₜ1 in eₜ2)
+    | tmc_expr_dir_call eₛ1 eₛ2 eₜ1 eₜ2 :
+        tmc_expr_dir eₛ1 eₜ1 →
+        tmc_expr_dir eₛ2 eₜ2 →
+        tmc_expr_dir
+          (eₛ1 eₛ2)
+          (eₜ1 eₜ2)
+    | tmc_expr_dir_unop op eₛ eₜ :
+        tmc_expr_dir eₛ eₜ →
+        tmc_expr_dir
+          (DataUnop op eₛ)
+          (DataUnop op eₜ)
+    | tmc_expr_dir_binop op eₛ1 eₛ2 eₜ1 eₜ2 :
+        tmc_expr_dir eₛ1 eₜ1 →
+        tmc_expr_dir eₛ2 eₜ2 →
+        tmc_expr_dir
+          (DataBinop op eₛ1 eₛ2)
+          (DataBinop op eₜ1 eₜ2)
+    | tmc_expr_dir_binop_det op eₛ1 eₛ2 eₜ1 eₜ2 :
+        tmc_expr_dir eₛ1 eₜ1 →
+        tmc_expr_dir eₛ2 eₜ2 →
+        tmc_expr_dir
+          (DataBinopDet op eₛ1 eₛ2)
+          (DataBinopDet op eₜ1 eₜ2)
+    | tmc_expr_dir_if eₛ0 eₛ1 eₛ2 eₜ0 eₜ1 eₜ2 :
+        tmc_expr_dir eₛ0 eₜ0 →
+        tmc_expr_dir eₛ1 eₜ1 →
+        tmc_expr_dir eₛ2 eₜ2 →
+        tmc_expr_dir
+          (if: eₛ0 then eₛ1 else eₛ2)
+          (if: eₜ0 then eₜ1 else eₜ2)
+    | tmc_expr_dir_block tag eₛ1 eₛ2 eₜ1 eₜ2 :
+        tmc_expr_dir eₛ1 eₜ1 →
+        tmc_expr_dir eₛ2 eₜ2 →
+        tmc_expr_dir
+          (&tag eₛ1 eₛ2)
+          (&tag eₜ1 eₜ2)
+    | tmc_expr_dir_block_dps_1 tag eₛ1 eₛ2 eₜ1 eₜ2 :
+        tmc_expr_dir eₛ1 eₜ1 →
+        tmc_expr_dps $0 𝟚 [] eₛ2.[ren (+1)] eₜ2 →
+        tmc_expr_dir
+          (&tag eₛ1 eₛ2)
+          (let: &tag eₜ1 #() in eₜ2 ;; $0)
+    | tmc_expr_dir_block_dps_2 tag eₛ1 eₛ2 eₜ1 eₜ2 :
+        tmc_expr_dir eₛ2 eₜ2 →
+        tmc_expr_dps $0 𝟙 [] eₛ1.[ren (+1)] eₜ1 →
+        tmc_expr_dir
+          (&tag eₛ1 eₛ2)
+          (let: &tag #() eₜ2 in eₜ1 ;; $0)
+    | tmc_expr_dir_block_dps tag eₛ1 eₛ2 eₜ1 eₜ2 eₜ :
+        tmc_expr_dps $0 𝟙 [] eₛ1.[ren (+1)] eₜ1 →
+        tmc_expr_dps $0 𝟚 [] eₛ2.[ren (+1)] eₜ2 →
+        eₜ = (let: &tag #() #() in eₜ1 ;; eₜ2 ;; $0)%data_expr →
+        tmc_expr_dir
+          (&tag eₛ1 eₛ2)
+          eₜ
+    | tmc_expr_dir_block_det tag eₛ1 eₛ2 eₜ1 eₜ2 :
+        tmc_expr_dir eₛ1 eₜ1 →
+        tmc_expr_dir eₛ2 eₜ2 →
+        tmc_expr_dir
+          (&&tag eₛ1 eₛ2)
+          (&&tag eₜ1 eₜ2)
+    | tmc_expr_dir_load eₛ1 eₛ2 eₜ1 eₜ2 :
+        tmc_expr_dir eₛ1 eₜ1 →
+        tmc_expr_dir eₛ2 eₜ2 →
+        tmc_expr_dir
+          (![eₛ2] eₛ1)
+          (![eₜ2] eₜ1)
+    | tmc_expr_dir_store eₛ1 eₛ2 eₛ3 eₜ1 eₜ2 eₜ3 :
+        tmc_expr_dir eₛ1 eₜ1 →
+        tmc_expr_dir eₛ2 eₜ2 →
+        tmc_expr_dir eₛ3 eₜ3 →
+        tmc_expr_dir
+          (eₛ1 <-[eₛ2]- eₛ3)
+          (eₜ1 <-[eₜ2]- eₜ3)
+  with tmc_expr_dps : data_expr → data_expr → tmc_ctx → data_expr → data_expr → Prop :=
+    | tmc_expr_dps_base dst idx C eₛ eₜ eₜ' :
+        tmc_expr_dir eₛ eₜ →
+        eₜ' = C @@ eₜ →
+        tmc_expr_dps dst idx C
+          eₛ
+          (dst <-[idx]- eₜ')
+    | tmc_expr_dps_let dst idx C eₛ1 eₛ2 eₜ1 eₜ2 :
+        tmc_expr_dir eₛ1 eₜ1 →
+        tmc_expr_dps dst.[ren (+1)] idx.[ren (+1)] C.|[ren (+1)] eₛ2 eₜ2 →
+        tmc_expr_dps dst idx C
+          (let: eₛ1 in eₛ2)
+          (let: eₜ1 in eₜ2)
+    | tmc_expr_dps_call dst idx func annot eₛ func_dps eₜ eₜ' :
+        ξ !! func = Some func_dps →
+        tmc_expr_dir eₛ eₜ →
+        eₜ' = (let: eₜ in (DataFunc func_dps annot) (dst.[ren (+1)], idx.[ren (+1)], $0))%data_expr →
+        tmc_expr_dps dst idx []
+          ((DataFunc func annot) eₛ)
+          eₜ'
+    | tmc_expr_dps_if dst idx C eₛ0 eₛ1 eₛ2 eₜ0 eₜ1 eₜ2 :
+        tmc_expr_dir eₛ0 eₜ0 →
+        tmc_expr_dps dst idx C eₛ1 eₜ1 →
+        tmc_expr_dps dst idx C eₛ2 eₜ2 →
+        tmc_expr_dps dst idx C
+          (if: eₛ0 then eₛ1 else eₛ2)
+          (if: eₜ0 then eₜ1 else eₜ2)
+    | tmc_expr_dps_block_1 dst idx C tag eₛ1 eₛ2 eₜ1 eₜ2 eₜ :
+        tmc_expr_dir eₛ1 eₜ1 →
+        tmc_expr_dps dst.[ren (+1)] idx.[ren (+1)] (TmcCtxi tag TmcRight $0 :: C.|[ren (+1)]) eₛ2.[ren (+1)] eₜ2 →
+        eₜ = (let: eₜ1 in eₜ2)%data_expr →
+        tmc_expr_dps dst idx C
+          (&tag eₛ1 eₛ2)
+          eₜ
+    | tmc_expr_dps_block_2 dst idx C tag eₛ1 eₛ2 eₜ1 eₜ2 eₜ :
+        tmc_expr_dir eₛ2 eₜ2 →
+        tmc_expr_dps dst.[ren (+1)] idx.[ren (+1)] (TmcCtxi tag TmcLeft $0 :: C.|[ren (+1)]) eₛ1.[ren (+1)] eₜ1 →
+        eₜ = (let: eₜ2 in eₜ1)%data_expr →
+        tmc_expr_dps dst idx C
+          (&tag eₛ1 eₛ2)
+          eₜ
+    | tmc_expr_dps_reify dst idx c C eₛ eₜ eₜ' :
+        tmc_expr_dps $0 c.(tmc_ctxi_side) [] eₛ.[ren (+1)] eₜ →
+        eₜ' = (let: c @@ #() in dst.[ren (+1)] <-[idx.[ren (+1)]]- (C.|[ren (+1)] @@ $0) ;; eₜ)%data_expr →
+        tmc_expr_dps dst idx (c :: C)
+          eₛ
+          eₜ'.
+End tmc_expr.
+
+Scheme tmc_expr_dir_dps_ind :=
+  Minimality for tmc_expr_dir Sort Prop
+with tmc_expr_dps_dir_ind :=
+  Minimality for tmc_expr_dps Sort Prop.
+Combined Scheme tmc_expr_ind from
+  tmc_expr_dir_dps_ind,
+  tmc_expr_dps_dir_ind.
+
+Create HintDb tmc.
+
+#[global] Hint Constructors tmc_expr_dir : tmc.
+#[global] Hint Constructors tmc_expr_dps : tmc.
+
+Record tmc {progₛ progₜ} := {
+  tmc_ξ : gmap data_function data_function ;
+
+  tmc_ξ_dom :
+    dom tmc_ξ ⊆ dom progₛ ;
+  tmc_dom :
+    dom progₜ = dom progₛ ∪ map_img tmc_ξ ;
+
+  tmc_dir func defₛ :
+    progₛ !! func = Some defₛ →
+      ∃ eₜ,
+      tmc_expr_dir tmc_ξ defₛ.(data_definition_body) eₜ ∧
+      progₜ !! func =
+        Some (
+          rec: defₛ.(data_definition_annot) :=
+            eₜ
+        )%data_def ;
+
+  tmc_dps func defₛ func_dps :
+    progₛ !! func = Some defₛ →
+    tmc_ξ !! func = Some func_dps →
+      ∃ eₜ,
+      tmc_expr_dps tmc_ξ $1 $2 [] defₛ.(data_definition_body) eₜ ∧
+      progₜ !! func_dps =
+        Some (
+          rec: defₛ.(data_definition_annot) :=
+            let: ![𝟙] $0 in
+            let: ![𝟚] $0 in
+            let: ![𝟙] $1 in
+            let: ![𝟚] $3 in
+            eₜ
+        )%data_def ;
+}.
+#[global] Arguments tmc : clear implicits.
