theories/tmc_2/metatheory.v
@@ -1,0 +1,354 @@
+From camlcert Require Import
+  prelude.
+From camlcert.data_lang Require Export
+  metatheory.
+From camlcert.tmc_2 Require Export
+  definition.
+From camlcert Require Import
+  options.
+
+Section tmc_ctxi.
+  Implicit Types c : tmc_ctxi.
+
+  Lemma tmc_ctxi_hsubst_comp c ς1 ς2 :
+    c.|[ς1].|[ς2] = c.|[ς1 >> ς2].
+  Proof.
+    destruct c as (?, [], ?); autosubst.
+  Qed.
+  Lemma tmc_ctxi_fill_subst c e ς :
+    (c @@ e).[ς] = c.|[ς] @@ e.[ς].
+  Proof.
+    destruct c as (?, [], ?); done.
+  Qed.
+
+  Definition tmc_ctxi_scoped scope c :=
+    data_expr_scoped scope c.(tmc_ctxi_expr).
+
+  Lemma tmc_ctxi_fill_scoped c e scope :
+    tmc_ctxi_scoped scope c →
+    data_expr_scoped scope e →
+    data_expr_scoped scope (c @@ e).
+  Proof.
+    destruct c as (?, [], ?); done.
+  Qed.
+  Lemma tmc_ctxi_scoped_lift1 scope c :
+    tmc_ctxi_scoped scope c →
+    tmc_ctxi_scoped (S scope) c.|[ren (+1)].
+  Proof.
+    destruct c as (?, [], ?); apply data_expr_scoped_lift1.
+  Qed.
+End tmc_ctxi.
+
+#[global] Hint Rewrite tmc_ctxi_hsubst_comp : autosubst.
+#[global] Hint Rewrite tmc_ctxi_fill_subst : autosubst.
+
+Section tmc_ctx.
+  Implicit Types C : tmc_ctx.
+
+  Lemma tmc_ctx_fill_nil e :
+    ([] : tmc_ctx) @@ e = e.
+  Proof.
+    done.
+  Qed.
+  Lemma tmc_ctx_fill_cons c C e :
+    (c :: C) @@ e = C @@ c @@ e.
+  Proof.
+    done.
+  Qed.
+  Lemma tmc_ctx_fill_app C1 C2 e :
+    (C1 ++ C2) @@ e = C2 @@ C1 @@ e.
+  Proof.
+    apply foldl_app.
+  Qed.
+  Lemma tmc_ctx_fill_snoc c C e :
+    (C ++ [c]) @@ e = c @@ C @@ e.
+  Proof.
+    rewrite tmc_ctx_fill_app //.
+  Qed.
+
+  Lemma tmc_ctx_hsubst_nil ς :
+    ([] : tmc_ctx).|[ς] = [].
+  Proof.
+    done.
+  Qed.
+  Lemma tmc_ctx_hsubst_cons c C ς :
+    (c :: C).|[ς] = c.|[ς] :: C.|[ς].
+  Proof.
+    done.
+  Qed.
+  Lemma tmc_ctx_hsubst_comp C ς1 ς2 :
+    C.|[ς1].|[ς2] = C.|[ς1 >> ς2].
+  Proof.
+    setoid_rewrite <- list_fmap_compose.
+    apply list_fmap_ext. intros. cbn.
+    rewrite tmc_ctxi_hsubst_comp //.
+  Qed.
+  Lemma tmc_ctx_fill_subst C e ς :
+    (C @@ e).[ς] = C.|[ς] @@ e.[ς].
+  Proof.
+    move: e. induction C as [| c C IH] => e; first done.
+    rewrite IH tmc_ctxi_fill_subst //.
+  Qed.
+
+  Definition tmc_ctx_scoped scope : tmc_ctx → Prop :=
+    Forall (tmc_ctxi_scoped scope).
+
+  Lemma tmc_ctx_scoped_nil scope :
+    tmc_ctx_scoped scope [].
+  Proof.
+    apply Forall_nil_2.
+  Qed.
+  Lemma tmc_ctx_scoped_cons scope c C :
+    tmc_ctxi_scoped scope c →
+    tmc_ctx_scoped scope C →
+    tmc_ctx_scoped scope (c :: C).
+  Proof.
+    apply Forall_cons_2.
+  Qed.
+  Lemma tmc_ctx_scoped_cons_inv scope c C :
+    tmc_ctx_scoped scope (c :: C) →
+      tmc_ctxi_scoped scope c ∧
+      tmc_ctx_scoped scope C.
+  Proof.
+    apply Forall_cons.
+  Qed.
+
+  Lemma tmc_ctx_fill_scoped C e scope :
+    tmc_ctx_scoped scope C →
+    data_expr_scoped scope e →
+    data_expr_scoped scope (C @@ e).
+  Proof.
+    move: e. induction C as [| c C IH] => e HC He; first done.
+    apply tmc_ctx_scoped_cons_inv in HC as (Hc & HC).
+    rewrite tmc_ctx_fill_cons.
+    apply IH; first done.
+    apply tmc_ctxi_fill_scoped; done.
+  Qed.
+  Lemma tmc_ctx_scoped_lift1 scope C :
+    tmc_ctx_scoped scope C →
+    tmc_ctx_scoped (S scope) C.|[ren (+1)].
+  Proof.
+    intros H.
+    apply Forall_fmap, (Forall_impl _ _ _ H), tmc_ctxi_scoped_lift1.
+  Qed.
+End tmc_ctx.
+
+#[global] Hint Rewrite tmc_ctx_hsubst_cons : autosubst.
+#[global] Hint Rewrite tmc_ctx_hsubst_comp : autosubst.
+#[global] Hint Rewrite tmc_ctx_fill_subst : autosubst.
+
+#[global] Hint Resolve tmc_ctx_scoped_nil : core.
+
+Section tmc_rctxi.
+  Implicit Types c : tmc_rctxi.
+
+  #[global] Instance tmc_rctxi_to_ctxi_inj :
+    Inj (=) (=) tmc_rctxi_to_ctxi.
+  Proof.
+    intros [] []. naive_solver.
+  Qed.
+
+  Lemma tmc_rctxi_hsubst c ς :
+    (c : tmc_ctxi).|[ς] = c.
+  Proof.
+    done.
+  Qed.
+End tmc_rctxi.
+
+#[global] Hint Rewrite tmc_rctxi_hsubst : autosubst.
+
+Section tmc_rctx.
+  Implicit Types C : tmc_rctx.
+
+  #[global] Instance tmc_rctx_to_ctx_inj :
+    Inj (=) (=) tmc_rctx_to_ctx.
+  Proof.
+    apply _.
+  Qed.
+
+  Lemma tmc_rctx_hsubst C ς :
+    (C : tmc_ctx).|[ς] = C.
+  Proof.
+    induction C as [| c C IH]; first done.
+    rewrite tmc_ctx_hsubst_cons tmc_rctxi_hsubst IH //.
+  Qed.
+End tmc_rctx.
+
+#[global] Hint Rewrite tmc_rctx_hsubst : autosubst.
+
+Section tmc_expr.
+  Context (ξ : tmc_mapping).
+
+  Lemma tmc_expr_dir_refl e :
+    tmc_expr_dir ξ e e.
+  Proof.
+    induction e; auto with tmc.
+  Qed.
+
+  Lemma tmc_expr_subst :
+    ( ∀ eₛ eₜ,
+      tmc_expr_dir ξ eₛ eₜ →
+      ∀ eₛ' eₜ' ς,
+      eₛ' = eₛ.[ς] →
+      eₜ' = eₜ.[ς] →
+      tmc_expr_dir ξ eₛ' eₜ'
+    ) ∧ (
+      ∀ dst idx C eₛ eₜ,
+      tmc_expr_dps ξ dst idx C eₛ eₜ →
+      ∀ dst' idx' C' eₛ' eₜ' ς,
+      dst' = dst.[ς] →
+      idx' = idx.[ς] →
+      C' = C.|[ς] →
+      eₛ' = eₛ.[ς] →
+      eₜ' = eₜ.[ς] →
+      tmc_expr_dps ξ dst' idx' C' eₛ' eₜ'
+    ).
+  Proof.
+    apply tmc_expr_ind; try solve
+    [ intros; simplify;
+      eauto using tmc_expr_dir_refl with tmc
+    | intros * ? ? ? IHdps **; simplify;
+      econstructor; try naive_solver; try apply IHdps with (up ς); autosubst
+    | intros * ? IHdps1 ? IHdps2 **; simplify;
+      econstructor;
+      [ apply IHdps1 with (up ς); autosubst
+      | apply IHdps2 with (up ς); autosubst
+      | autosubst
+      ]
+    ].
+    - intros. simplify.
+      econstructor; [naive_solver | asimpl; done].
+    - intros * ? IHdps **. simplify.
+      econstructor; first apply IHdps with (up ς); autosubst.
+  Qed.
+  Lemma tmc_expr_dir_subst ς eₛ eₛ' eₜ eₜ' :
+    tmc_expr_dir ξ eₛ eₜ →
+    eₛ' = eₛ.[ς] →
+    eₜ' = eₜ.[ς] →
+    tmc_expr_dir ξ eₛ' eₜ'.
+  Proof.
+    eauto using (proj1 tmc_expr_subst).
+  Qed.
+  Lemma tmc_expr_dps_subst ς dst dst' idx idx' C C' eₛ eₛ' eₜ eₜ' :
+    tmc_expr_dps ξ dst idx C eₛ eₜ →
+    dst' = dst.[ς] →
+    idx' = idx.[ς] →
+    eₛ' = eₛ.[ς] →
+    eₜ' = eₜ.[ς] →
+    C' = C.|[ς] →
+    tmc_expr_dps ξ dst' idx' C' eₛ' eₜ'.
+  Proof.
+    eauto using (proj2 tmc_expr_subst).
+  Qed.
+
+  Lemma data_expr_scoped_tmc_expr :
+    ( ∀ eₛ eₜ,
+      tmc_expr_dir ξ eₛ eₜ →
+      ∀ scope,
+      data_expr_scoped scope eₛ →
+      data_expr_scoped scope eₜ
+    ) ∧ (
+      ∀ dst idx C eₛ eₜ,
+      tmc_expr_dps ξ dst idx C eₛ eₜ →
+      ∀ scope,
+      data_expr_scoped scope dst →
+      data_expr_scoped scope idx →
+      tmc_ctx_scoped scope C →
+      data_expr_scoped scope eₛ →
+      data_expr_scoped scope eₜ
+    ).
+  Proof.
+    apply tmc_expr_ind; try naive_solver.
+    - intros * Hdir1 IH1 Hdps2 IH2 scope (Hscoped1 & Hscoped2).
+      simpl. split_and!; try naive_solver lia.
+      apply IH2; try naive_solver auto with lia.
+      apply data_expr_scoped_lift1. done.
+    - intros * Hdir2 IH2 Hdps1 IH1 scope (Hscoped1 & Hscoped2).
+      simpl. split_and!; try naive_solver lia.
+      apply IH1; try naive_solver auto with lia.
+      apply data_expr_scoped_lift1. done.
+    - intros * Hdps1 IH1 Hdps2 IH2 -> scope (Hscoped1 & Hscoped2).
+      simpl. split_and!; try lia.
+      + apply IH1; try naive_solver auto with lia.
+        apply data_expr_scoped_lift1. done.
+      + apply data_expr_scoped_lift1.
+        apply IH2; try naive_solver auto with lia.
+        apply data_expr_scoped_lift1. done.
+    - intros * Hdir IH -> scope Hdst Hidx HC Heₛ.
+      split_and!; try naive_solver.
+      auto using tmc_ctx_fill_scoped.
+    - intros * Hdir1 IH1 Hdps2 IH2 scope Hdst Hidx HC (Hscoped1 & Hscoped2).
+      split; first auto.
+      apply IH2; try done.
+      + apply data_expr_scoped_lift1. done.
+      + apply data_expr_scoped_lift1. done.
+      + apply tmc_ctx_scoped_lift1. done.
+    - intros * Hξ Hdir IH -> scope Hdst Hidx HC (_ & Hscoped).
+      simpl. split_and!; [eauto using data_expr_scoped_lift1.. | lia].
+    - intros * Hdir1 IH1 Hdps2 IH2 -> scope Hdst Hidx HC (Hscoped1 & Hscoped2).
+      split; first auto.
+      apply IH2; try done.
+      + apply data_expr_scoped_lift1. done.
+      + apply data_expr_scoped_lift1. done.
+      + apply tmc_ctx_scoped_cons.
+        * cbn. lia.
+        * apply tmc_ctx_scoped_lift1. done.
+      + apply data_expr_scoped_lift1. done.
+    - intros * Hdir1 IH1 Hdps2 IH2 -> scope Hdst Hidx HC (Hscoped1 & Hscoped2).
+      split; first auto.
+      apply IH2; try done.
+      + apply data_expr_scoped_lift1. done.
+      + apply data_expr_scoped_lift1. done.
+      + apply tmc_ctx_scoped_cons.
+        * cbn. lia.
+        * apply tmc_ctx_scoped_lift1. done.
+      + apply data_expr_scoped_lift1. done.
+    - intros * Hdps IH -> scope Hdst Hidx (Hc & HC)%tmc_ctx_scoped_cons_inv Heₛ.
+      simpl. split_and!.
+      + apply tmc_ctxi_fill_scoped; done.
+      + apply data_expr_scoped_lift1. done.
+      + apply data_expr_scoped_lift1. done.
+      + apply tmc_ctx_fill_scoped.
+        * apply tmc_ctx_scoped_lift1. done.
+        * simpl. lia.
+      + apply data_expr_scoped_lift1, IH; try naive_solver auto with lia.
+        apply data_expr_scoped_lift1. done.
+  Qed.
+  Lemma data_expr_scoped_tmc_expr_dir scope eₛ eₜ :
+    tmc_expr_dir ξ eₛ eₜ →
+    data_expr_scoped scope eₛ →
+    data_expr_scoped scope eₜ.
+  Proof.
+    eauto using (proj1 data_expr_scoped_tmc_expr).
+  Qed.
+  Lemma data_expr_scoped_tmc_expr_dps scope dst idx C eₛ eₜ :
+    tmc_expr_dps ξ dst idx C eₛ eₜ →
+    data_expr_scoped scope dst →
+    data_expr_scoped scope idx →
+      tmc_ctx_scoped scope C →
+    data_expr_scoped scope eₛ →
+    data_expr_scoped scope eₜ.
+  Proof.
+    eauto using (proj2 data_expr_scoped_tmc_expr).
+  Qed.
+End tmc_expr.
+
+#[global] Hint Resolve tmc_expr_dir_refl : tmc.
+
+Lemma data_program_scoped_tmc progₛ progₜ :
+  tmc progₛ progₜ →
+  data_program_scoped progₛ →
+  data_program_scoped progₜ.
+Proof.
+  intros tmc. rewrite /data_program_scoped !map_Forall_lookup. intros Hscoped func defₜ Hfuncₜ.
+  apply elem_of_dom_2 in Hfuncₜ as Hfuncₜ'. rewrite tmc.(tmc_dom) elem_of_union in Hfuncₜ'.
+  destruct Hfuncₜ' as [Hfuncₛ%lookup_lookup_total_dom | (func_dir & Hξ)%elem_of_map_img].
+  - edestruct tmc.(tmc_dir) as (eₜ & Hdir & Heq); first done.
+    eapply data_expr_scoped_tmc_expr_dir; last naive_solver.
+    rewrite Heq in Hfuncₜ. naive_solver.
+  - pose proof Hξ as Hfunc_dirₛ%elem_of_dom_2%(tmc.(tmc_ξ_dom))%lookup_lookup_total_dom.
+    edestruct tmc.(tmc_dps) as (eₜ & Hdps & Heq); [done.. |].
+    rewrite Hfuncₜ in Heq. simplify.
+    repeat constructor. eapply data_expr_scoped_tmc_expr_dps; [naive_solver.. |].
+    apply (data_expr_scoped_le 1); naive_solver lia.
+Qed.
